move castR and castD + cosmetics

theories/Views/ProdView.v
@@ -1,15 +1,9 @@
 Require Import ExtLib.Core.RelDec.
 Require Import ExtLib.Data.Fun.
-Require Import ExtLib.Data.Map.FMapPositive.
-Require Import ExtLib.Data.SumN.
-Require Import ExtLib.Data.Positive.
-Require Import ExtLib.Tactics.Consider.
 Require Import ExtLib.Tactics.
 Require Import ExtLib.Relations.TransitiveClosure.
 
 Require Import MirrorCore.TypesI.
-Require Import MirrorCore.syms.SymEnv.
-Require Import MirrorCore.syms.SymSum.
 Require Import MirrorCore.Lambda.Expr.
 Require Import MirrorCore.Lambda.Ptrns.
 Require Import MirrorCore.Views.Ptrns.
@@ -26,10 +20,10 @@ Section TypeOfSymAs.
   Context {typ func : Type}.
   Context {RType_typ : RType typ}.
   Context {RSym_func : RSym func}.
-  
+
   Lemma typeof_sym_symAs (s : func) t v (H : symAs s t = Some v) : typeof_sym s = Some t.
   Proof.
-    unfold symAs in H. 
+    unfold symAs in H.
     generalize dependent (symD s).
     forward.
   Qed.
@@ -47,10 +41,10 @@ Section ProdFuncInst.
   Context {typ func : Type} {RType_typ : RType typ}.
   Context {RelDec_typ : RelDec (@eq typ)}.
   Context {RelDecCorrect_typ : RelDec_Correct RelDec_typ}.
-  
+
   Context {Typ2_tyArr : Typ2 _ Fun}.
   Context {Typ2_tyProd : Typ2 _ prod}.
-  
+
   Let tyArr : typ -> typ -> typ := @typ2 _ _ _ Typ2_tyArr.
   Let tyProd : typ -> typ -> typ := @typ2 _ _ _ Typ2_tyProd.
 
@@ -60,7 +54,7 @@ Section ProdFuncInst.
       | pFst t1 t2 => Some (tyArr (tyProd t1 t2) t1)
       | pSnd t1 t2 => Some (tyArr (tyProd t1 t2) t2)
     end.
-  
+
   Definition prod_func_eq (a b : prod_func typ) : option bool :=
     match a , b with
       | pPair t1 t2, pPair t3 t4 => Some (t1 ?[ eq ] t3 &&
@@ -72,24 +66,7 @@ Section ProdFuncInst.
       | _, _ => None
     end.
 
-  Definition castD F U {T : Typ0 _ U} (val : F (typD (typ0 (F:=U)))) : F U :=
-    match @typ0_cast typ _ _ T in _ = x return F x with
-      | eq_refl => val
-    end.
-
-  Definition castR F U {T : Typ0 _ U} (val : F U) : F (typD (typ0 (F:=U))) :=
-    match eq_sym (@typ0_cast typ _ _ T) in _ = x return F x with
-    | eq_refl => val
-    end.
-
-  Existing Instance Typ2_App.
-  Existing Instance Typ1_App.
-  Existing Instance Typ0_term.
-
-  Implicit Arguments castD [[T]].
-  Implicit Arguments castR [[T]].
-
-  Definition pairD t u : typD (tyArr t (tyArr u (tyProd t u))) -> 
+  Definition pairD t u : typD (tyArr t (tyArr u (tyProd t u))) ->
                          Fun (typD t) (Fun (typD u) (typD t * typD u)) :=
     castD id (Fun (typD t) (Fun (typD u) (typD t * typD u)%type)).
 
@@ -104,10 +81,10 @@ Section ProdFuncInst.
 
   Definition sndD t u : typD (tyArr (tyProd t u) u) -> Fun (typD t * typD u) (typD u) :=
     castD id (Fun (typD t * typD u) (typD u)).
-  
+
   Definition sndR t u : typD (tyArr (tyProd t u) u) :=
     castR id (Fun (typD t * typD u) (typD u)) snd.
-  
+
   Definition prod_func_symD bf :=
     match bf as bf return match typeof_prod_func bf return Type with
 			    | Some t => typD t
@@ -119,13 +96,13 @@ Section ProdFuncInst.
     end.
 
   Global Instance RSym_ProdFunc
-  : SymI.RSym (prod_func typ) := 
+  : SymI.RSym (prod_func typ) :=
     {
       typeof_sym := typeof_prod_func;
       symD := prod_func_symD ;
       sym_eqb := prod_func_eq
     }.
-  
+
   Global Instance RSymOk_ProdFunc : SymI.RSymOk RSym_ProdFunc.
   Proof.
     split; intros.
@@ -137,7 +114,7 @@ Section ProdFuncInst.
     + consider (t ?[ eq ] t1 && t0 ?[ eq ] t2)%bool;
       intuition congruence.
   Qed.
-  
+
 End ProdFuncInst.
 
 Implicit Arguments castD [[RType_typ] [T]].
@@ -160,26 +137,26 @@ Section MakeProd.
 
   Definition fptrnPair {T : Type} (p : Ptrns.ptrn (typ * typ) T) : ptrn (prod_func typ) T :=
     fun f U good bad =>
-      match f with 
+      match f with
         | pPair t u => p (t, u) U good (fun x => bad f)
         | _ => bad f
       end.
 
   Definition fptrnFst {T : Type} (p : Ptrns.ptrn (typ * typ) T) : ptrn (prod_func typ) T :=
     fun f U good bad =>
-      match f with 
+      match f with
         | pFst t u => p (t, u) U good (fun x => bad f)
         | _ => bad f
       end.
 
   Definition fptrnSnd {T : Type} (p : Ptrns.ptrn (typ * typ) T) : ptrn (prod_func typ) T :=
     fun f U good bad =>
-      match f with 
+      match f with
         | pSnd t u => p (t, u) U good (fun x => bad f)
         | _ => bad f
       end.
 
-  Global Instance fptrnPair_ok {T : Type} {p : ptrn (typ * typ) T} {Hok : ptrn_ok p} : 
+  Global Instance fptrnPair_ok {T : Type} {p : ptrn (typ * typ) T} {Hok : ptrn_ok p} :
     ptrn_ok (fptrnPair p).
   Proof.
     red; intros.
@@ -190,8 +167,8 @@ Section MakeProd.
     { right; unfold Fails; reflexivity. }
     { right; unfold Fails; reflexivity. }
   Qed.
-     
-  Global Instance fptrnFst_ok {T : Type} {p : ptrn (typ * typ) T} {Hok : ptrn_ok p} : 
+
+  Global Instance fptrnFst_ok {T : Type} {p : ptrn (typ * typ) T} {Hok : ptrn_ok p} :
     ptrn_ok (fptrnFst p).
   Proof.
     red; intros.
@@ -202,8 +179,8 @@ Section MakeProd.
     { right; unfold Fails in *; intros; simpl; rewrite H; reflexivity. }
     { right; unfold Fails; reflexivity. }
   Qed.
-     
-  Global Instance fptrnSnd_ok {T : Type} {p : ptrn (typ * typ) T} {Hok : ptrn_ok p} : 
+
+  Global Instance fptrnSnd_ok {T : Type} {p : ptrn (typ * typ) T} {Hok : ptrn_ok p} :
     ptrn_ok (fptrnSnd p).
   Proof.
     red; intros.
@@ -215,23 +192,23 @@ Section MakeProd.
     { right; unfold Fails in *; intros; simpl; rewrite H; reflexivity. }
   Qed.
 
-  Definition ptrnPair {A B T : Type} 
+  Definition ptrnPair {A B T : Type}
              (p : ptrn (typ * typ) T)
              (a : ptrn (expr typ func) A)
              (b : ptrn (expr typ func) B) : ptrn (expr typ func) (A * B) :=
-    pmap (fun x => match x with | (_, a, b) => (a, b) end) 
+    pmap (fun x => match x with | (_, a, b) => (a, b) end)
          (app (app (inj (ptrn_view _ (fptrnPair p))) a) b).
 
-  Definition ptrnFst {A T : Type} 
+  Definition ptrnFst {A T : Type}
              (p : ptrn (typ * typ) T)
              (a : ptrn (expr typ func) A) : ptrn (expr typ func) A :=
     pmap snd (app (inj (ptrn_view _ (fptrnFst p))) a).
 
-  Definition ptrnSnd {A T : Type} 
+  Definition ptrnSnd {A T : Type}
              (p : ptrn (typ * typ) T)
              (a : ptrn (expr typ func) A) : ptrn (expr typ func) A :=
     pmap snd (app (inj (ptrn_view _ (fptrnSnd p))) a).
-  
+
   Lemma Succeeds_fptrnPair {T : Type} (f : prod_func typ) (p : ptrn (typ * typ) T) (res : T)
         {pok : ptrn_ok p} (H : Succeeds f (fptrnPair p) res) :
     exists t u, Succeeds (t, u) p res /\ f = pPair t u.
@@ -246,7 +223,7 @@ Section MakeProd.
     rewrite H0 in H; inv_all; subst.
     exists t, t0; split; [assumption | reflexivity].
   Qed.
-  
+
   Lemma Succeeds_fptrnFst {T : Type} (f : prod_func typ) (p : ptrn (typ * typ) T) (res : T)
         {pok : ptrn_ok p} (H : Succeeds f (fptrnFst p) res) :
     exists t u, Succeeds (t, u) p res /\ f = pFst t u.
@@ -261,7 +238,7 @@ Section MakeProd.
     rewrite H0 in H; inv_all; subst.
     exists t, t0; split; [assumption | reflexivity].
   Qed.
-  
+
   Lemma Succeeds_fptrnSnd {T : Type} (f : prod_func typ) (p : ptrn (typ * typ) T) (res : T)
         {pok : ptrn_ok p} (H : Succeeds f (fptrnSnd p) res) :
     exists t u, Succeeds (t, u) p res /\ f = pSnd t u.
@@ -276,7 +253,7 @@ Section MakeProd.
     rewrite H0 in H; inv_all; subst.
     exists t, t0; split; [assumption | reflexivity].
   Qed.
-  
+
 End MakeProd.
 
 Section Tactics.
@@ -295,7 +272,7 @@ Section Tactics.
 
   Let tyArr := @typ2 _ _ _ Typ2_tyArr.
   Let tyProd := @typ2 _ _ _ Typ2_tyProd.
-  
+
   Definition red_fst_ptrn : ptrn (expr typ func) (expr typ func) :=
     pmap (fun xy => fst xy) (ptrnFst ignore (ptrnPair ignore get ignore)).
 
@@ -306,29 +283,26 @@ Section Tactics.
 
   Definition red_snd := run_tptrn (pdefault_id red_snd_ptrn).
 
-  Definition FST := SIMPLIFY (typ := typ) 
-                             (fun _ _ _ _ => 
+  Definition FST := SIMPLIFY (typ := typ)
+                             (fun _ _ _ _ =>
                                 (beta_all (fun _ e args => red_fst (apps e args)))).
 
   Ltac destruct_prod :=
-    match goal with 
+    match goal with
       | p : ?A * ?B |- _ => destruct p; destruct_prod
       | _ => idtac
     end.
 
-  Existing Instance Typ2_App.
-  Existing Instance Typ1_App.
-  Existing Instance Typ0_term.
   Existing Instance MirrorCore.ExprI.Applicative_exprT.
 
-Require Import MirrorCore.Util.Compat.
+  Require Import MirrorCore.Util.Compat.
 
-Theorem exprT_App_Fun tus tvs T U (T0 : Typ0 _ T) (U0 : Typ0 _ U)
-        (e1 : exprT tus tvs (Fun T U))
-        (e2 : exprT tus tvs T) :
-@exprT_App typ _ Typ2_tyArr tus tvs (@typ0 _ _ T _) (@typ0 _ _ U _) (@castR typ _ (exprT tus tvs) _ _ e1)
-                 (@castR typ _ (exprT tus tvs) _ _ e2) =
-      @castR typ _ (exprT tus tvs) U U0 (Applicative.ap e1 e2).
+  Theorem exprT_App_Fun tus tvs T U (T0 : Typ0 _ T) (U0 : Typ0 _ U)
+          (e1 : exprT tus tvs (Fun T U))
+          (e2 : exprT tus tvs T) :
+    @exprT_App typ _ Typ2_tyArr tus tvs (@typ0 _ _ T _) (@typ0 _ _ U _) (@castR typ _ (exprT tus tvs) _ _ e1)
+               (@castR typ _ (exprT tus tvs) _ _ e2) =
+    @castR typ _ (exprT tus tvs) U U0 (Applicative.ap e1 e2).
   Proof.
     unfold exprT_App. simpl. intros.
     unfold castR. simpl.
@@ -345,17 +319,17 @@ Theorem exprT_App_Fun tus tvs T U (T0 : Typ0 _ T) (U0 : Typ0 _ U)
     destruct (eq_sym e). simpl. reflexivity.*)
   Admitted.
 
-Theorem exprT_App_Fun' tus tvs T U (T0 : Typ0 _ T) (U0 : Typ0 _ U)  P
-        (e1 : exprT tus tvs (Fun T U))
-        (e2 : exprT tus tvs T) 
-        (Hres : P (@castR typ _ (exprT tus tvs) U U0 (Applicative.ap e1 e2))) :
-  P (@exprT_App typ _ Typ2_tyArr tus tvs (@typ0 _ _ T _) (@typ0 _ _ U _) (@castR typ _ (exprT tus tvs) _ _ e1) (@castR typ _ (exprT tus tvs) _ _ e2)).
+  Theorem exprT_App_Fun' tus tvs T U (T0 : Typ0 _ T) (U0 : Typ0 _ U)  P
+          (e1 : exprT tus tvs (Fun T U))
+          (e2 : exprT tus tvs T)
+          (Hres : P (@castR typ _ (exprT tus tvs) U U0 (Applicative.ap e1 e2))) :
+    P (@exprT_App typ _ Typ2_tyArr tus tvs (@typ0 _ _ T _) (@typ0 _ _ U _) (@castR typ _ (exprT tus tvs) _ _ e1) (@castR typ _ (exprT tus tvs) _ _ e2)).
   Proof.
     subst. rewrite exprT_App_Fun. assumption.
   Qed.
 
   Lemma exprT_App_castR_pure {A : Type} {T0 : Typ0 RType_typ A} tus tvs (f : exprT tus tvs A) :
-    (fun us vs => castR typ id A (f us vs)) = 
+    (fun us vs => castR typ id A (f us vs)) =
     (castR typ (exprT tus tvs) A f).
   Proof.
     unfold castR, eq_sym; simpl.
@@ -365,194 +339,151 @@ Theorem exprT_App_Fun' tus tvs T U (T0 : Typ0 _ T) (U0 : Typ0 _ U)  P
   Admitted.
 
 
-    Ltac force_apply lem :=
-      let L := fresh "L" in 
-      pose proof lem as L; apply L; clear L.
+  Ltac force_apply lem :=
+    let L := fresh "L" in
+    pose proof lem as L; apply L; clear L.
 
-Ltac ptrn_prod_sound_step :=
-  match goal with
-    | H : Succeeds _ (fptrnPair _) _ |- _ => 
-      apply Succeeds_fptrnPair in H; destruct H as [? [? ?]]; repeat subst
-    | H : Succeeds _ (fptrnFst _) _ |- _ => 
-      apply Succeeds_fptrnFst in H; destruct H as [? [? ?]]; repeat subst
-    | H : Succeeds _ (fptrnSnd _) _ |- _ => 
-      apply Succeeds_fptrnSnd in H; destruct H as [? [? ?]]; repeat subst
-end.
-
-Ltac ptrn_sound_step :=
-  first [
-      ptrn_base_sound_step |
-      ptrn_prod_sound_step
-    ].
-
-Class SucceedsE {X T : Type} (f : X) (p : ptrn X T) (v : T) := {
-  s_result : Prop;
-  s_elim : Succeeds f p v -> s_result
-}.
-
-Global Instance fptrnPair_SucceedsE {T : Type} {f : prod_func typ} {p : ptrn (typ * typ) T} {res : T} {pok : ptrn_ok p} :
-
-  SucceedsE f (fptrnPair p) res := {
-  s_result := exists t u, Succeeds (t, u) p res /\ f = pPair t u;
-  s_elim := @Succeeds_fptrnPair typ T f p res  pok
-}.
-
-Global Instance fptrnFst_SucceedsE {T : Type} {f : prod_func typ} {p : ptrn (typ * typ) T} {res : T} {pok : ptrn_ok p} :
-
-  SucceedsE f (fptrnFst p) res := {
-  s_result := exists t u, Succeeds (t, u) p res /\ f = pFst t u;
-  s_elim := @Succeeds_fptrnFst typ T f p res pok
-}.
-
-Global Instance fptrnSnd_SucceedsE {T : Type} {f : prod_func typ} {p : ptrn (typ * typ) T} {res : T} {pok : ptrn_ok p} :
-
-  SucceedsE f (fptrnSnd p) res := {
-  s_result := exists t u, Succeeds (t, u) p res /\ f = pSnd t u;
-  s_elim := @Succeeds_fptrnSnd typ T f p res  pok
-}.
-
-Global Instance pmap_SucceedsE {X T U : Type} {x : X} {f : T -> U} {p : ptrn X T} {res : U} 
-         {pok : ptrn_ok p} : 
-  SucceedsE x (pmap f p) res := {
-  s_result := exists y, Succeeds x p y /\ res = f y;
-  s_elim := Succeeds_pmap pok
-}.
-
-Global Instance app_SucceedsE {T U : Type} {e : expr typ func} 
-       {p : ptrn (expr typ func) T} {q : ptrn (expr typ func) U} {res : T * U} 
-         {pok_p : ptrn_ok p} {pok_q : ptrn_ok q} :
-  SucceedsE e (app p q) res := {
-  s_result := exists l r, e = App l r /\ Succeeds l p (fst res) /\ Succeeds r q (snd res);
-  s_elim := Succeeds_app pok_p pok_q
-}.
-
-Global Instance inj_SucceedsE {T : Type} {e : expr typ func} 
-       {p : ptrn func T}  {res : T} 
-         {pok_p : ptrn_ok p} :
-  SucceedsE e (inj p) res := {
-  s_result := exists f, e = Inj f /\ Succeeds f p res;
-  s_elim := Succeeds_inj pok_p
-}.
-
-Global Instance get_SucceedsE {X : Type} {x res : X} :
-  SucceedsE x get res := {
-  s_result := x = res;
-  s_elim := @Succeeds_get X x res 
-}.
-
-Global Instance ignore_SucceedsE {X : Type} {x : X} (res : unit) :
-  SucceedsE x ignore res := {
-  s_result := res = tt;
-  s_elim := 
-    fun _ => match res as x return (x = tt) with
-               | tt => eq_refl
-             end
-}.
-
-Global Instance ptrn_view_SucceedsE {A T : Type} {x : func} {res : T} {p : ptrn A T} 
-       {FV : FuncView func A} {Sym_A : RSym A} {FVOk : FuncViewOk FV _ Sym_A}
-       {pok : ptrn_ok p} :
-  SucceedsE x (ptrn_view FV p) res := {
-  s_result := exists f : A, f_insert f = x /\ Succeeds f p res;
-  s_elim := @Succeeds_ptrn_view func A FV typ _ _ _ _ _ p x res _
-}.
-
-
-Ltac ptrn_elim :=
-  repeat
-   match goal with
-   | H:Succeeds ?f ?p ?v
-     |- _ =>
-         let z := constr:(_:SucceedsE f p v) in
-         apply s_elim in H; do 2 red in H; destruct_ands H
-   end.
-
-Ltac exprT_App_red :=
+  Ltac ptrn_prod_sound_step :=
     match goal with
-      | |- context [castR _ id _ _] => rewrite exprT_App_castR_pure
-      | |- context [@exprT_App _ _ _ ?tus ?tvs _ _ (castR _ _ (Fun ?t1 ?t2) _) ?v] =>
+    | H : Succeeds _ (fptrnPair _) _ |- _ =>
+      apply Succeeds_fptrnPair in H; destruct H as [? [? ?]]; repeat subst
+    | H : Succeeds _ (fptrnFst _) _ |- _ =>
+      apply Succeeds_fptrnFst in H; destruct H as [? [? ?]]; repeat subst
+    | H : Succeeds _ (fptrnSnd _) _ |- _ =>
+      apply Succeeds_fptrnSnd in H; destruct H as [? [? ?]]; repeat subst
+    end.
 
-        first [
-            force_apply (@exprT_App_Fun' tus tvs t1 t2 _ _) |
-            replace v with (castR typ (exprT tus tvs) _ v) by reflexivity;
-              force_apply (@exprT_App_Fun' tus tvs t1 t2 _ _)
-          ]
-    end. 
+  Class SucceedsE {X T : Type} (f : X) (p : ptrn X T) (v : T) :=
+  { s_result : Prop
+  ; s_elim : Succeeds f p v -> s_result }.
 
-Check @exprD'.
-Require Import ExprD.
-Class ExprDE tus tvs (e : expr typ func) (t : typ) (v : exprT tus tvs (typD t)) := {
-  e_result : Prop;
-  e_elim : exprD' tus tvs t e = Some v -> e_result
-}.
+  Global Instance fptrnPair_SucceedsE {T : Type} {f : prod_func typ} {p : ptrn (typ * typ) T} {res : T} {pok : ptrn_ok p}
+  : SucceedsE f (fptrnPair p) res :=
+  { s_result := exists t u, Succeeds (t, u) p res /\ f = pPair t u
+  ; s_elim := @Succeeds_fptrnPair typ T f p res  pok }.
 
-Instance Injective_exprD'_App tus tvs (e1 e2 : expr typ func) (t : typ) (v : exprT tus tvs (typD t)):
-  Injective (exprD' tus tvs t (App e1 e2) = Some v) := {
-    result := exists u v1 v2, exprD' tus tvs (tyArr u t) e1 = Some v1 /\
+  Global Instance fptrnFst_SucceedsE {T : Type} {f : prod_func typ} {p : ptrn (typ * typ) T} {res : T} {pok : ptrn_ok p}
+  : SucceedsE f (fptrnFst p) res :=
+  { s_result := exists t u, Succeeds (t, u) p res /\ f = pFst t u
+  ; s_elim := @Succeeds_fptrnFst typ T f p res pok }.
+
+  Global Instance fptrnSnd_SucceedsE {T : Type} {f : prod_func typ} {p : ptrn (typ * typ) T} {res : T} {pok : ptrn_ok p}
+  : SucceedsE f (fptrnSnd p) res :=
+  { s_result := exists t u, Succeeds (t, u) p res /\ f = pSnd t u
+  ; s_elim := @Succeeds_fptrnSnd typ T f p res  pok }.
+
+  Global Instance pmap_SucceedsE {X T U : Type} {x : X} {f : T -> U} {p : ptrn X T} {res : U} {pok : ptrn_ok p}
+  : SucceedsE x (pmap f p) res :=
+  { s_result := exists y, Succeeds x p y /\ res = f y
+  ; s_elim := Succeeds_pmap pok }.
+
+  Global Instance app_SucceedsE {T U : Type} {e : expr typ func}
+         {p : ptrn (expr typ func) T} {q : ptrn (expr typ func) U} {res : T * U}
+         {pok_p : ptrn_ok p} {pok_q : ptrn_ok q}
+  : SucceedsE e (app p q) res :=
+  { s_result := exists l r, e = App l r /\ Succeeds l p (fst res) /\ Succeeds r q (snd res)
+  ; s_elim := Succeeds_app pok_p pok_q }.
+
+  Global Instance inj_SucceedsE {T : Type} {e : expr typ func}
+         {p : ptrn func T}  {res : T}
+         {pok_p : ptrn_ok p}
+  : SucceedsE e (inj p) res :=
+  { s_result := exists f, e = Inj f /\ Succeeds f p res
+  ; s_elim := Succeeds_inj pok_p }.
+
+  Global Instance get_SucceedsE {X : Type} {x res : X}
+  : SucceedsE x get res :=
+  { s_result := x = res
+  ; s_elim := @Succeeds_get X x res }.
+
+  Global Instance ignore_SucceedsE {X : Type} {x : X} (res : unit)
+  : SucceedsE x ignore res :=
+  { s_result := res = tt
+  ; s_elim :=
+      fun _ => match res as x return (x = tt) with
+               | tt => eq_refl
+               end }.
+
+  Global Instance ptrn_view_SucceedsE {A T : Type} {x : func} {res : T} {p : ptrn A T}
+       {FV : FuncView func A} {Sym_A : RSym A} {FVOk : FuncViewOk FV _ Sym_A}
+       {pok : ptrn_ok p}
+  : SucceedsE x (ptrn_view FV p) res :=
+  { s_result := exists f : A, f_insert f = x /\ Succeeds f p res
+  ; s_elim := @Succeeds_ptrn_view func A FV typ _ _ _ _ _ p x res _ }.
+
+
+  Ltac ptrn_elim :=
+    repeat
+      match goal with
+      | H:Succeeds ?f ?p ?v
+        |- _ =>
+        let z := constr:(_:SucceedsE f p v) in
+        apply s_elim in H; do 2 red in H; destruct_ands H
+      end.
+
+  Ltac exprT_App_red :=
+    match goal with
+    | |- context [castR _ id _ _] => rewrite exprT_App_castR_pure
+    | |- context [@exprT_App _ _ _ ?tus ?tvs _ _ (castR _ _ (Fun ?t1 ?t2) _) ?v] =>
+
+      first [
+          force_apply (@exprT_App_Fun' tus tvs t1 t2 _ _) |
+          replace v with (castR typ (exprT tus tvs) _ v) by reflexivity;
+            force_apply (@exprT_App_Fun' tus tvs t1 t2 _ _)
+        ]
+    end.
+
+  Require Import MirrorCore.Lambda.ExprD.
+
+  Class ExprDE tus tvs (e : expr typ func) (t : typ) (v : exprT tus tvs (typD t)) :=
+  { e_result : Prop
+  ; e_elim : exprD' tus tvs t e = Some v -> e_result }.
+
+  Instance Injective_exprD'_App tus tvs (e1 e2 : expr typ func) (t : typ) (v : exprT tus tvs (typD t))
+  : Injective (exprD' tus tvs t (App e1 e2) = Some v) :=
+  { result := exists u v1 v2, exprD' tus tvs (tyArr u t) e1 = Some v1 /\
                               exprD' tus tvs u e2 = Some v2 /\
                               v = exprT_App v1 v2;
     injection := fun H => _
-}.
-Proof.
-  autorewrite with exprD_rw in H.
-  simpl in H. forward; inv_all; subst.
-  do 3 eexists; repeat split; eassumption.
-Defined.
+  }.
+  Proof.
+    autorewrite with exprD_rw in H.
+    simpl in H. forward; inv_all; subst.
+    do 3 eexists; repeat split; eassumption.
+  Defined.
 
-Instance Injective_exprD'_Inj tus tvs (f : func) (t : typ) (v : exprT tus tvs (typD t)):
-  Injective (exprD' tus tvs t (Inj f) = Some v) := {
-    result := exists v', symAs f t = Some v' /\ v = fun _ _ => v';
-    injection := fun H => _
-}.
-Proof.
-  autorewrite with exprD_rw in H.
-  simpl in H. forward; inv_all; subst.
-  eexists; repeat split.
-Defined.
-Instance Injective_exprD'_f_insert {A : Type} (a : A) (t : typ) (v : typD t) 
-         {FV : FuncView func A} {RSym_A : RSym A}  {FVOk : FuncViewOk _ _ RSym_A} :
-  Injective (symAs (f_insert a) t = Some v) := {
-    result := symAs a t = Some v;
-    injection := fun H => _
-}.
-Proof.
-  rewrite fv_compat; assumption.
-Defined.
-Check Relim.
-Definition symAs' := symAs.
-Lemma test : @symAs' = @symAs.
-Proof.
-  reflexivity.
-Qed.
-Opaque symAs'.
-(*
-Instance Injective_pPair (a b c : typ) v : Injective (symAs (pPair a b) c = Some v) := {
-  result := exists r : c = (tyArr a (tyArr b (tyProd a b))), v = Relim id r (pairR a b);
-  injection := fun H => _
-}.
-Proof.
-  unfold symAs in H.
-  simpl in H. 
-  forward.
-  unfold Rty in r; subst.
-  inv_all; subst. eexists; split.
-Defined.
-*)
+  Instance Injective_exprD'_Inj tus tvs (f : func) (t : typ) (v : exprT tus tvs (typD t))
+  : Injective (exprD' tus tvs t (Inj f) = Some v) :=
+  { result := exists v', symAs f t = Some v' /\ v = fun _ _ => v'
+  ; injection := fun H => _ }.
+  Proof.
+    autorewrite with exprD_rw in H.
+    simpl in H. forward; inv_all; subst.
+    eexists; repeat split.
+  Defined.
 
+  Instance Injective_exprD'_f_insert {A : Type} (a : A) (t : typ) (v : typD t)
+           {FV : FuncView func A} {RSym_A : RSym A}  {FVOk : FuncViewOk _ _ RSym_A}
+  : Injective (symAs (f_insert a) t = Some v) :=
+  { result := symAs a t = Some v
+  ; injection := fun H => _ }.
+  Proof.
+    rewrite fv_compat; assumption.
+  Defined.
 
-    Ltac symAsE := 
-      match goal with
-        | H : symAs ?f ?t = Some ?v |- _ =>
-          let Heq := fresh "Heq" in
-          pose proof (typeof_sym_symAs _ _ H) as Heq;
-            simpl in Heq; inv_all; repeat subst;
-            unfold symAs in H; simpl in H; rewrite type_cast_refl in H; [|apply _];
-            simpl in H; inv_all; subst
-      end.
+  Ltac symAsE :=
+    match goal with
+    | H : symAs ?f ?t = Some ?v |- _ =>
+      let Heq := fresh "Heq" in
+      pose proof (typeof_sym_symAs _ _ H) as Heq;
+        simpl in Heq; inv_all; repeat subst;
+        unfold symAs in H; simpl in H; rewrite type_cast_refl in H; [|apply _];
+        simpl in H; inv_all; subst
+    end.
 
-Ltac ptrnE :=
-  ptrn_elim; destruct_prod; simpl in *; subst; inv_all; repeat subst;
-  repeat symAsE.
+  Ltac ptrnE :=
+    ptrn_elim; destruct_prod; simpl in *; subst; inv_all; repeat subst;
+    repeat symAsE.
 
   Lemma red_fst_ok : partial_reducer_ok (fun e args => red_fst (apps e args)).
   Proof.
@@ -560,7 +491,6 @@ Ltac ptrnE :=
     exists val; split; [|reflexivity].
     generalize dependent (apps e es); clear e es; intros e H.
     unfold red_fst.
-    
     apply run_tptrn_id_sound; [assumption|]; intros.
     ptrnE.
     unfold pairR, fstR.
